add once to coqproject

theories/once.v
@@ -1,25 +1,27 @@
 From det Require Import prelude.
 From mathcomp Require Import all_ssreflect.
 From det Require Import tree tree_prop ctx.
-From det Require Import tree_prop_hard.
+From det Require Import tree_prop_hard tree_vars mut_excl unif.
 
 From det Require Import check_fo.
 
 Lemma is_det_tail_cut u p s fv l:
-  is_det u p s fv (And l [::cut] (And (TA cut) [::] OK)).
+  is_det u p s fv (And l [::cut] (TA cut)).
 Proof.
-  move=> b s' tx fv' H.
+  move=> r [s'[r' H]].
   remember (And _ _ _) as t' eqn:Ht'.
   elim_run H l Ht'.
-  - by move: SA; rewrite rew_pa => /andP[]//.
+  - by move: sA; rewrite rew_pa => /andP[]//.
   - move: pA eA; rewrite rew_pa/= !push.
     case: ifP => sl pA [???]; subst.
     rewrite -success_cut in sl.
-    inversion rB; subst => //=.
+    inversion rB; subst; simpl in *; eauto.
     - rewrite sl prune_cutl//.
-    - move: H0 => /=; rewrite sl => -[???]; subst.
-      by move: H; rewrite rew_pa sl//.
-    - move: H; rewrite rew_pa sl success_failed//.
+    - rewrite/=; eauto.
+    - move: H0; rewrite/=sl => -[???]; subst.
+      by move: H; rewrite rew_pa sl.
+    - move: H0; rewrite sl => -[?]; subst.
+      by move: H; rewrite rew_pa success_failed//=sl.
   - by apply: IH erefl.
   - move: fA nA; rewrite rew_pa/=.
     move=> /orP[fl|/andP[]]//.
@@ -46,8 +48,11 @@ Section once.
 
   Definition no_once (r: seq R) :=
     forall x, x \in r -> 
-      if callable (head x) is Some hd then hd <> once_sym
+      if get_tm_hd (head x) is inl hd then hd <> once_sym
       else true.
+
+  Lemma no_once_cons x xs: no_once (x :: xs) -> no_once xs.
+  Proof. by rewrite/no_once/= => H r H1; apply/H; rewrite in_cons H1 orbT. Qed.
 
   Definition prog_once p :=
     (p.(sig) = p.(sig) + once_sigS) /\ forall r, 
@@ -57,32 +62,39 @@ Section once.
     (sig + once_sigS).[? once_sym] = Some once_sig.
   Proof. by rewrite/once_sigS !FmapE.fmapE eqxx/= fsetU0 in_fset1 eqxx. Qed.
 
-  Lemma bc_once u rs s t sig: no_once rs ->
-    let fv := (vars_tm t `|` vars_sigma s) in
-    exists x y, (bc u {| rules := once_impl :: rs; sig := sig + once_sigS |} fv
-    (Tm_App (Tm_P once_sym) t) s).2 = 
-     ([::(x, call y :: cut :: [::])]).
-  Proof.
-    rewrite/bc [callable _]/=.
-    case X: fresh_rules => [fv' rs'].
-    rewrite /=!FmapE.fmapE/= fsetU0 in_fset1 eqxx.
-    case Y: select => [fv2 rs2]/=.
-    move: X; rewrite/=!push => -[??]; subst.
-    move: Y.
-    rewrite !cat0f.
-    set X := ren _ _.
-    set Y := ren _ _.
-    rewrite/=eqxx/= in_fnd/=; first by rewrite in_fset1.
-    move=> H + NR.
-    rewrite ffunE. erewrite (valPE H).
-    rewrite ffunE fset0U codomf0 fsetU0.
+  Lemma get_modes_rev_once_sym t:
+    get_modes_rev (Tm_App (Tm_P once_sym) t) once_sig = [:: i].
+  Proof. by []. Qed.
 
-    case M: matching => /=.
-      rewrite !push/= => -[??]; subst.
-      repeat eexists; f_equal.
-      admit.
-    admit.
-  Admitted.
+  Lemma no_once_select u t rs s:
+    no_once rs ->
+    select u (Tm_App (Tm_P once_sym) t) [:: i] rs s = (fset0, [::]).
+  Proof.
+    elim: rs t s => //= -[hd bo] xs IH t s/= H1.
+    have {}IH := IH _ _ (no_once_cons H1).
+    rewrite IH/=.
+    destruct hd => //=; case: eqP => //= Hz; subst.
+    move: H1; rewrite /no_once.
+    set P := {|head := _; premises := _|}.
+    by move=> /(_ P); rewrite in_cons eqxx => /(_ isT).
+  Qed.
+
+  Lemma no_once_fresh fv rs: no_once rs -> no_once (fresh_rules fv rs).2.
+  Proof.
+    rewrite/no_once/=. 
+    elim: rs fv => //= x xs IH fv H e; rewrite !push/=.
+    rewrite in_cons => /orP[/eqP?|]; subst; last first.
+      apply/IH => H1 H2; apply/H.
+      by rewrite in_cons H2 orbT.
+    rewrite/fresh_rule!push/=.
+    case: x H => /= hd bo H.
+    rewrite/rename !push/=.
+    set X := fresh_tm _ _ _.
+    case Y: get_tm_hd => //=[p].
+    have:= callable_ren X.2 hd p; rewrite Y => /proj1/(_ erefl) H1.
+    have:= H (mkR hd bo); rewrite/= in_cons H1 eqxx; auto.
+  Qed.
+
 
   Lemma id_det_once u p s t:
     prog_once p ->
@@ -90,26 +102,45 @@ Section once.
   Proof.
     case: p => -[|r rs] sig []//= HS; first by move=> /(_ [::]) [].
     move=> /(_ rs) [[?] H]; subst.
-    rewrite/is_det HS => b s' t' fv' Hx.
+    rewrite/is_det HS => r' [b'[fv' Hx]].
     inversion Hx; clear Hx; subst => //.
-    move: H1; rewrite/= !push/= => -[???]; subst.
-    move: H3.
-    set PR := {|rules := _; sig := _|}.
-    have [x[y Hx]] := bc_once u s t sig H.
-    rewrite Hx => Hy; inversion Hy; clear Hy; subst => //.
-    rewrite rew_pa in H1.
-    move: H2 => /= => -[?]; subst.
-    inversion H3; clear H3; subst => //.
-    move: H4; rewrite/=!push/=.
-    set BC := bc _ _ _ _ _.
-    set A:= And _ _ _.
+    move: H1; rewrite/=/bc [get_tm_hd _]/=.
+    cbn iota.
+    rewrite once_sigP/=.
+    case X: fresh_rules => [fvx' rs'].
+    rewrite/fresh_rule/= fset0U codomf0/= fsetU0/rename cat0f.
+    rewrite/fresh_tm inE eqxx get_modes_rev_once_sym ren_app ren_V ren_P.
+    rewrite in_fnd; first by rewrite inE.
+    have:= fresh_rules_sub rs (vars_tm t `|` vars_sigma s).
+    rewrite X => /= HH.
+    move=> H1/=; rewrite eqxx/= ffunE matching_V//=; last first.
+      apply/fsubset_trans.
+        apply/mut_excl.vars_deref/fsubsetUr.
+        apply/fsubsetUl.
+        by apply/fsubset_trans/fsubsetUr.
+      move: HH; rewrite fsubUset => /andP[_ Hx].
+      by apply/fsubset_trans/fsubsetUr.
+    rewrite no_once_select//=.
+    rewrite/vars_sigma/= /varsU_rule/varsU_rhead/varsU_rprem/= fset0U/=.
+    rewrite !fsetUA/= !fsetU0.
+    rewrite !(fsetUC _ fvx') !fsetUA.
+    rewrite !(fsetUC _ [fset IV 0]) !fsetUA fsetUid.
+    rewrite !(fsetUC _ [fset fresh _]) !fsetUA !fsetUid.
     move=> [???]; subst.
-    have:= run_same_structure H6.
-    destruct t' => //=; destruct t0 => //= /andP[/eqP?/eqP?]; subst.
-    have ? := run_or0 H6; subst.
-    have/=:= run_ko_left2 u PR BC.1 fv' s0 A (Some t0) s' s.
-    move=> /proj2/(_ H6) [b1 Hr].
-    by have:= is_det_tail_cut Hr.
+    have:= run_or0 H3 => ?; subst.
+    have:= run_ko_ONK H3.
+    case: r' H3 => [[s1 t1]|] H3; last by eauto.
+    have /= := run_same_structure H3.
+    case: t1 H3 => [[]|]//=; last by eauto.
+    move=> l sm r H3 /andP[/eqP?/eqP?]; subst.
+    move=> /(_ (Some (s1, Some r)) erefl).
+    move=> [b] Hz.
+    have {}Hz := ex_intro _ _ Hz.
+    have {}Hz := ex_intro (fun x => exists y, runT _ _ _ _ _ _ x _) _ Hz.
+    have:= is_det_tail_cut Hz.
+    by move=> [|[]]//.
+    move: X; rewrite [fresh_rules _ _]surjective_pairing => -[_ <-].
+    by apply: no_once_fresh.
   Qed.
 
 
